projection/proofs/to_cake/ffi/comms_ffi_rec_characScript.sml
@@ -1,0 +1,632 @@
+open HolKernel boolLib Parse bossLib;
+open optionTheory
+     relationTheory
+     listTheory
+     rich_listTheory;
+open ffiTheory;
+open payloadSemTheory
+     payloadLangTheory
+     payloadPropsTheory
+     payloadConfluenceTheory
+     bisimulationTheory
+     bisimulation_extTheory
+     comms_ffi_modelTheory
+     comms_ffi_consTheory
+     comms_ffi_propsTheory
+     comms_ffi_commTheory
+     comms_ffi_eqTheory;
+
+val _ = new_theory "comms_ffi_rec_charac";
+(* General Hilbert Choice Helper *)
+Theorem some_satisfies_cond:
+  ∀P. (some x. P x) = SOME z ⇒ P z
+Proof
+  rw[some_def] >> SELECT_ELIM_TAC >>
+  metis_tac[]
+QED
+
+(* FFI State Receive property *)
+Definition ffi_receives_def:
+  ffi_receives conf st src msg =
+    ((conf.payload_size > 0) ∧
+    (LENGTH msg > 0) ∧
+    (∀s param bytes.
+      conf.payload_size > 0 ∧
+      LENGTH msg > 0 ∧
+      valid_receive_call_format conf src s param bytes ⇒
+      ∃nst nbytes.
+          call_FFI st s param bytes = FFI_return nst nbytes ∧
+          nbytes = pad conf msg ∧
+          (final nbytes ∨
+           (intermediate nbytes ∧
+            ffi_receives conf nst src (DROP conf.payload_size msg)))))
+Termination
+  WF_REL_TAC ‘measure (λ(_,_,_,msg). LENGTH msg)’ >>
+  rw[]
+End
+
+Theorem ffi_eq_receives:
+  ∀conf x y.
+    ffi_wf x.ffi_state ∧
+    ffi_wf y.ffi_state ∧
+    x.oracle = comms_ffi_oracle conf ∧
+    y.oracle = comms_ffi_oracle conf ∧
+    ffi_eq conf x.ffi_state y.ffi_state ⇒
+    ffi_receives conf x = ffi_receives conf y
+Proof
+  simp[FUN_EQ_THM,PULL_FORALL] >>
+  rpt gen_tac >>
+  rename1 ‘ffi_receives conf x src msg = ffi_receives conf y src msg’ >>
+  MAP_EVERY qid_spec_tac [‘y’,‘x’] >>
+  completeInduct_on ‘LENGTH msg’ >>
+  rw[Once ffi_receives_def] >>
+  qmatch_goalsub_abbrev_tac ‘LP ⇔ _’ >>
+  rw[Once ffi_receives_def] >>
+  qunabbrev_tac ‘LP’ >>
+  qmatch_goalsub_abbrev_tac ‘PA ∧ PB ∧ PCA ⇔ PA ∧ PB ∧ PCB’ >>
+  ‘PCA ⇔ PCB’
+    suffices_by rw[] >>
+  MAP_EVERY qunabbrev_tac [‘PA’,‘PB’,‘PCA’,‘PCB’] >>
+  rw[EQ_IMP_THM] >>
+  first_x_assum (drule_all_then strip_assume_tac) >>
+  rw[]
+  >- (rfs[call_FFI_def,valid_receive_call_format_def,
+         comms_ffi_oracle_def,ffi_receive_def] >>
+      DEEP_INTRO_TAC some_intro >> rw[] >>
+      Cases_on ‘some (m,ns). (strans conf x.ffi_state (ARecv param m) ns)’ >>
+      fs[] >>
+      rename1 ‘(some (m,ns). strans conf x.ffi_state (ARecv param m) ns) = SOME nsb’ >>
+      ‘(λ(m,ns). strans conf x.ffi_state (ARecv param m) ns) nsb’
+            by metis_tac[some_satisfies_cond] >>
+      PairCases_on ‘nsb’ >> fs[]
+      >- (rename1 ‘(λ(m,ns). strans conf y.ffi_state (ARecv param m) ns) ns’ >>
+          PairCases_on ‘ns’ >>
+          Cases_on ‘LENGTH ns0 = SUC conf.payload_size’ >> fs[] >>
+          ‘nsb0 = ns0’
+            by metis_tac[ffi_eq_ARecv] >>
+          fs[])
+      >- (rw[pairTheory.EXISTS_PROD] >>
+          qexists_tac ‘nsb0’ >>
+          rw[GSYM pairTheory.EXISTS_PROD] >>
+          qabbrev_tac ‘L = ARecv param nsb0’ >>
+          qabbrev_tac ‘x2 = (nsb1,nsb2,nsb3)’ >>
+          metis_tac[ffi_eq_def,BISIM_REL_def,BISIM_def]))
+  >- (rfs[call_FFI_def,valid_receive_call_format_def,
+         comms_ffi_oracle_def,ffi_receive_def] >>
+      DEEP_INTRO_TAC some_intro >> rw[] >>
+      Cases_on ‘some (m,ns). (strans conf x.ffi_state (ARecv param m) ns)’ >>
+      fs[] >>
+      rename1 ‘(some (m,ns). strans conf x.ffi_state (ARecv param m) ns) = SOME nsb’ >>
+      ‘(λ(m,ns). strans conf x.ffi_state (ARecv param m) ns) nsb’
+            by metis_tac[some_satisfies_cond] >>
+      PairCases_on ‘nsb’ >> fs[]
+      >- (rename1 ‘(λ(m,ns). strans conf y.ffi_state (ARecv param m) ns) ns’ >>
+          PairCases_on ‘ns’ >> fs[] >>
+          ‘nsb0 = ns0’
+            by metis_tac[ffi_eq_ARecv] >>
+          fs[] >> Cases_on ‘LENGTH ns0 = SUC conf.payload_size’ >> fs[] >>
+          DISJ2_TAC >>
+          last_x_assum (qspec_then ‘LENGTH (DROP conf.payload_size msg)’ assume_tac) >>
+          rfs[] >> first_x_assum (qspec_then ‘DROP conf.payload_size msg’ assume_tac) >>
+          rfs[] >> qmatch_goalsub_abbrev_tac ‘ffi_receives _ nstY _ _’ >>
+          first_x_assum (qspecl_then [‘nst’,‘nstY’] assume_tac) >>
+          rfs[] >> pop_assum irule >>
+          qunabbrev_tac ‘nstY’ >>
+          qpat_x_assum ‘_ = nst’ (SUBST1_TAC o GSYM) >>
+          rw[] >> metis_tac[strans_pres_wf,ffi_eq_pres])
+      >- (rw[pairTheory.EXISTS_PROD] >>
+          qexists_tac ‘nsb0’ >>
+          rw[GSYM pairTheory.EXISTS_PROD] >>
+          qabbrev_tac ‘L = ARecv param nsb0’ >>
+          qabbrev_tac ‘x2 = (nsb1,nsb2,nsb3)’ >>
+          metis_tac[ffi_eq_def,BISIM_REL_def,BISIM_def]))
+  >- (rfs[call_FFI_def,valid_receive_call_format_def,
+         comms_ffi_oracle_def,ffi_receive_def] >>
+      DEEP_INTRO_TAC some_intro >> rw[] >>
+      Cases_on ‘some (m,ns). (strans conf y.ffi_state (ARecv param m) ns)’ >>
+      fs[] >>
+      rename1 ‘(some (m,ns). strans conf y.ffi_state (ARecv param m) ns) = SOME nsb’ >>
+      ‘(λ(m,ns). strans conf y.ffi_state (ARecv param m) ns) nsb’
+            by metis_tac[some_satisfies_cond] >>
+      PairCases_on ‘nsb’ >> fs[]
+      >- (rename1 ‘(λ(m,ns). strans conf x.ffi_state (ARecv param m) ns) ns’ >>
+          PairCases_on ‘ns’ >>
+          Cases_on ‘LENGTH ns0 = SUC conf.payload_size’ >> fs[] >>
+          ‘nsb0 = ns0’
+            by metis_tac[ffi_eq_ARecv] >>
+          fs[])
+      >- (rw[pairTheory.EXISTS_PROD] >>
+          qexists_tac ‘nsb0’ >>
+          rw[GSYM pairTheory.EXISTS_PROD] >>
+          qabbrev_tac ‘L = ARecv param nsb0’ >>
+          qabbrev_tac ‘y2 = (nsb1,nsb2,nsb3)’ >>
+          metis_tac[ffi_eq_def,BISIM_REL_def,BISIM_def]))
+  >- (rfs[call_FFI_def,valid_receive_call_format_def,
+         comms_ffi_oracle_def,ffi_receive_def] >>
+      DEEP_INTRO_TAC some_intro >> rw[] >>
+      Cases_on ‘some (m,ns). (strans conf y.ffi_state (ARecv param m) ns)’ >>
+      fs[] >>
+      rename1 ‘(some (m,ns). strans conf y.ffi_state (ARecv param m) ns) = SOME nsb’ >>
+      ‘(λ(m,ns). strans conf y.ffi_state (ARecv param m) ns) nsb’
+            by metis_tac[some_satisfies_cond] >>
+      PairCases_on ‘nsb’ >> fs[]
+      >- (rename1 ‘(λ(m,ns). strans conf x.ffi_state (ARecv param m) ns) ns’ >>
+          PairCases_on ‘ns’ >> fs[] >>
+          ‘nsb0 = ns0’
+            by metis_tac[ffi_eq_ARecv] >>
+          fs[] >> Cases_on ‘LENGTH ns0 = SUC conf.payload_size’ >> fs[] >>
+          DISJ2_TAC >>
+          last_x_assum (qspec_then ‘LENGTH (DROP conf.payload_size msg)’ assume_tac) >>
+          rfs[] >> first_x_assum (qspec_then ‘DROP conf.payload_size msg’ assume_tac) >>
+          rfs[] >> qmatch_goalsub_abbrev_tac ‘ffi_receives _ nstX _ _’ >>
+          first_x_assum (qspecl_then [‘nst’,‘nstX’] assume_tac) >>
+          rfs[] >> pop_assum irule >>
+          qunabbrev_tac ‘nstX’ >>
+          qpat_x_assum ‘_ = nst’ (SUBST1_TAC o GSYM) >>
+          rw[] >>
+          metis_tac[strans_pres_wf,ffi_eq_pres,ffi_eq_equivRel,
+                    equivalence_def,symmetric_def])
+      >- (rw[pairTheory.EXISTS_PROD] >>
+          qexists_tac ‘nsb0’ >>
+          rw[GSYM pairTheory.EXISTS_PROD] >>
+          qabbrev_tac ‘L = ARecv param nsb0’ >>
+          qabbrev_tac ‘y2 = (nsb1,nsb2,nsb3)’ >>
+          metis_tac[ffi_eq_def,BISIM_REL_def,BISIM_def]))
+QED
+
+Definition ffi_term_stream_def:
+  (ffi_term_stream conf st src (c1::c2::cs) =
+    (¬final c1 ∧
+    ∀s param bytes.
+      valid_receive_call_format conf src s param bytes ⇒
+      ∃nst.
+        call_FFI st s param bytes = FFI_return nst c1 ∧
+        ffi_term_stream conf nst src (c2::cs))) ∧
+  (ffi_term_stream conf st src (c1::[]) =
+    (final c1 ∧
+    ∀s param bytes.
+      valid_receive_call_format conf src s param bytes ⇒
+      ∃nst.
+        call_FFI st s param bytes = FFI_return nst c1)) ∧
+  (ffi_term_stream conf st src [] = F)
+End
+
+Theorem ffi_eq_term_stream:
+  ∀conf x y.
+    ffi_wf x.ffi_state ∧
+    ffi_wf y.ffi_state ∧
+    x.oracle = comms_ffi_oracle conf ∧
+    y.oracle = comms_ffi_oracle conf ∧
+    ffi_eq conf x.ffi_state y.ffi_state ⇒
+    ffi_term_stream conf x = ffi_term_stream conf y
+Proof
+  simp[FUN_EQ_THM,PULL_FORALL] >>
+  rpt gen_tac >>
+  rename1 ‘ffi_term_stream conf x src chnks = ffi_term_stream conf y src chnks’ >>
+  MAP_EVERY qid_spec_tac [‘y’,‘x’] >>
+  Induct_on ‘chnks’
+  >- rw[ffi_term_stream_def] >>
+  Cases_on ‘chnks’ >>
+  rw[ffi_term_stream_def] >>
+  irule (DECIDE “∀a b c. (b ⇔ c) ⇒ ((a ∧ b) ⇔ (a ∧ c))”) >>
+  rw[EQ_IMP_THM] >>
+  first_x_assum (drule_all_then strip_assume_tac)
+  >- (rfs[call_FFI_def,valid_receive_call_format_def,
+         comms_ffi_oracle_def,ffi_receive_def] >>
+      DEEP_INTRO_TAC some_intro >> rw[] >>
+      Cases_on ‘some (m,ns). (strans conf x.ffi_state (ARecv param m) ns)’ >>
+      fs[] >>
+      rename1 ‘(some (m,ns). strans conf x.ffi_state (ARecv param m) ns) = SOME nsb’ >>
+      ‘(λ(m,ns). strans conf x.ffi_state (ARecv param m) ns) nsb’
+            by metis_tac[some_satisfies_cond] >>
+      PairCases_on ‘nsb’ >> fs[]
+      >- (rename1 ‘(λ(m,ns). strans conf y.ffi_state (ARecv param m) ns) ns’ >>
+          PairCases_on ‘ns’ >>
+          Cases_on ‘LENGTH ns0 = SUC conf.payload_size’ >> fs[] >>
+          ‘nsb0 = ns0’
+            by metis_tac[ffi_eq_ARecv] >>
+          fs[])
+      >- (rw[pairTheory.EXISTS_PROD] >>
+          qexists_tac ‘nsb0’ >>
+          rw[GSYM pairTheory.EXISTS_PROD] >>
+          qabbrev_tac ‘L = ARecv param nsb0’ >>
+          qabbrev_tac ‘x2 = (nsb1,nsb2,nsb3)’ >>
+          metis_tac[ffi_eq_def,BISIM_REL_def,BISIM_def]))
+  >- (rfs[call_FFI_def,valid_receive_call_format_def,
+         comms_ffi_oracle_def,ffi_receive_def] >>
+      DEEP_INTRO_TAC some_intro >> rw[] >>
+      Cases_on ‘some (m,ns). (strans conf y.ffi_state (ARecv param m) ns)’ >>
+      fs[] >>
+      rename1 ‘(some (m,ns). strans conf y.ffi_state (ARecv param m) ns) = SOME nsb’ >>
+      ‘(λ(m,ns). strans conf y.ffi_state (ARecv param m) ns) nsb’
+            by metis_tac[some_satisfies_cond] >>
+      PairCases_on ‘nsb’ >> fs[]
+      >- (rename1 ‘(λ(m,ns). strans conf x.ffi_state (ARecv param m) ns) ns’ >>
+          PairCases_on ‘ns’ >>
+          Cases_on ‘LENGTH ns0 = SUC conf.payload_size’ >> fs[] >>
+          ‘nsb0 = ns0’
+            by metis_tac[ffi_eq_ARecv] >>
+          fs[])
+      >- (rw[pairTheory.EXISTS_PROD] >>
+          qexists_tac ‘nsb0’ >>
+          rw[GSYM pairTheory.EXISTS_PROD] >>
+          qabbrev_tac ‘L = ARecv param nsb0’ >>
+          qabbrev_tac ‘x2 = (nsb1,nsb2,nsb3)’ >>
+          metis_tac[ffi_eq_def,BISIM_REL_def,BISIM_def]))
+  >- (rfs[call_FFI_def,valid_receive_call_format_def,
+         comms_ffi_oracle_def,ffi_receive_def] >>
+      DEEP_INTRO_TAC some_intro >> rw[] >>
+      Cases_on ‘some (m,ns). (strans conf x.ffi_state (ARecv param m) ns)’ >>
+      fs[] >>
+      rename1 ‘(some (m,ns). strans conf x.ffi_state (ARecv param m) ns) = SOME nsb’ >>
+      ‘(λ(m,ns). strans conf x.ffi_state (ARecv param m) ns) nsb’
+            by metis_tac[some_satisfies_cond] >>
+      PairCases_on ‘nsb’ >> fs[]
+      >- (rename1 ‘(λ(m,ns). strans conf y.ffi_state (ARecv param m) ns) ns’ >>
+          PairCases_on ‘ns’ >> fs[] >>
+          ‘nsb0 = ns0’
+            by metis_tac[ffi_eq_ARecv] >>
+          fs[] >> Cases_on ‘LENGTH ns0 = SUC conf.payload_size’ >> fs[] >>
+          qmatch_goalsub_abbrev_tac ‘ffi_term_stream conf nstY param (h::t)’ >>
+          ‘ffi_term_stream conf nst param (h::t) ⇔
+           ffi_term_stream conf nstY param (h::t)’
+            suffices_by metis_tac[] >>
+          last_x_assum irule >>
+          qunabbrev_tac ‘nstY’ >> fs[] >>
+          qpat_x_assum ‘_ = nst’ (fn x => REWRITE_TAC[GSYM x]) >>
+          rw[]
+          >- metis_tac[strans_pres_wf]
+          >- metis_tac[strans_pres_wf]
+          >- metis_tac[ffi_eq_pres])
+      >- (rw[pairTheory.EXISTS_PROD] >>
+          qexists_tac ‘nsb0’ >>
+          rw[GSYM pairTheory.EXISTS_PROD] >>
+          qabbrev_tac ‘L = ARecv param nsb0’ >>
+          qabbrev_tac ‘x2 = (nsb1,nsb2,nsb3)’ >>
+          metis_tac[ffi_eq_def,BISIM_REL_def,BISIM_def]))
+  >- (rfs[call_FFI_def,valid_receive_call_format_def,
+         comms_ffi_oracle_def,ffi_receive_def] >>
+      DEEP_INTRO_TAC some_intro >> rw[] >>
+      Cases_on ‘some (m,ns). (strans conf y.ffi_state (ARecv param m) ns)’ >>
+      fs[] >>
+      rename1 ‘(some (m,ns). strans conf y.ffi_state (ARecv param m) ns) = SOME nsb’ >>
+      ‘(λ(m,ns). strans conf y.ffi_state (ARecv param m) ns) nsb’
+            by metis_tac[some_satisfies_cond] >>
+      PairCases_on ‘nsb’ >> fs[]
+      >- (rename1 ‘(λ(m,ns). strans conf x.ffi_state (ARecv param m) ns) ns’ >>
+          PairCases_on ‘ns’ >> fs[] >>
+          ‘nsb0 = ns0’
+            by metis_tac[ffi_eq_ARecv] >>
+          fs[] >> Cases_on ‘LENGTH ns0 = SUC conf.payload_size’ >> fs[] >>
+          qmatch_goalsub_abbrev_tac ‘ffi_term_stream conf nstX param (h::t)’ >>
+          ‘ffi_term_stream conf nst param (h::t) ⇔
+           ffi_term_stream conf nstX param (h::t)’
+            suffices_by metis_tac[] >>
+          last_x_assum irule >>
+          qunabbrev_tac ‘nstX’ >> fs[] >>
+          qpat_x_assum ‘_ = nst’ (fn x => REWRITE_TAC[GSYM x]) >>
+          rw[]
+          >- metis_tac[strans_pres_wf]
+          >- metis_tac[strans_pres_wf]
+          >- metis_tac[ffi_eq_equivRel,equivalence_def,symmetric_def,
+                       ffi_eq_pres])
+      >- (rw[pairTheory.EXISTS_PROD] >>
+          qexists_tac ‘nsb0’ >>
+          rw[GSYM pairTheory.EXISTS_PROD] >>
+          qabbrev_tac ‘L = ARecv param nsb0’ >>
+          qabbrev_tac ‘x2 = (nsb1,nsb2,nsb3)’ >>
+          metis_tac[ffi_eq_def,BISIM_REL_def,BISIM_def]))
+QED
+
+Definition ffi_divg_stream_def:
+  (ffi_divg_stream conf st src (c1::cs) =
+    (¬final c1 ∧
+    ∀s param bytes.
+      valid_receive_call_format conf src s param bytes ⇒
+      ∃nst.
+        call_FFI st s param bytes = FFI_return nst c1 ∧
+        ffi_divg_stream conf nst src cs)) ∧
+  (ffi_divg_stream conf st src [] =
+    ∀s param bytes.
+      valid_receive_call_format conf src s param bytes ⇒
+        call_FFI st s param bytes = FFI_final(Final_event s param bytes FFI_diverged))
+End
+
+Theorem ffi_eq_divg_stream:
+  ∀conf x y.
+    ffi_wf x.ffi_state ∧
+    ffi_wf y.ffi_state ∧
+    x.oracle = comms_ffi_oracle conf ∧
+    y.oracle = comms_ffi_oracle conf ∧
+    ffi_eq conf x.ffi_state y.ffi_state ⇒
+    ffi_divg_stream conf x = ffi_divg_stream conf y
+Proof
+  simp[FUN_EQ_THM,PULL_FORALL] >>
+  rpt gen_tac >>
+  rename1 ‘ffi_divg_stream conf x src chnks = ffi_divg_stream conf y src chnks’ >>
+  MAP_EVERY qid_spec_tac [‘y’,‘x’] >>
+  Induct_on ‘chnks’
+  >- (rw[ffi_divg_stream_def,EQ_IMP_THM] >>
+      first_x_assum (drule_all_then strip_assume_tac) >>
+      rfs[call_FFI_def,ffi_receive_def,valid_receive_call_format_def,
+         comms_ffi_oracle_def,AllCaseEqs()] >>
+      first_x_assum mp_tac >>
+      ntac 2 (DEEP_INTRO_TAC some_intro) >>
+      rw[pairTheory.EXISTS_PROD] >>
+      rename1 ‘(λ(m,ns). strans _ _ (ARecv param m) ns) XP’ >>
+      PairCases_on ‘XP’ >>
+      fs[] >> qexists_tac ‘XP0’ >>
+      rw[GSYM pairTheory.EXISTS_PROD] >>
+      qabbrev_tac ‘XP = (XP1,XP2,XP3)’ >>
+      first_x_assum (K ALL_TAC) >>
+      metis_tac[ffi_eq_def,BISIM_REL_def,BISIM_def]) >>
+  rw[ffi_divg_stream_def, EQ_IMP_THM] >>
+  first_x_assum (drule_all_then strip_assume_tac) >>
+  rfs[call_FFI_def,ffi_receive_def,valid_receive_call_format_def,
+         comms_ffi_oracle_def,AllCaseEqs()] >>
+  qpat_x_assum ‘(some (m,ns). strans conf _ (ARecv _ m) ns) = _’ mp_tac >>
+  ntac 2 (DEEP_INTRO_TAC some_intro) >>
+  rw[pairTheory.EXISTS_PROD]
+  >- (rename1 ‘(λ(m,ns). strans _ _ (ARecv param m) ns) XP’ >>
+      PairCases_on ‘XP’ >>
+      fs[] >> rw[]
+      >- metis_tac[ffi_eq_ARecv] >>
+      qmatch_asmsub_abbrev_tac  ‘ffi_divg_stream conf nstX param chnks’ >>
+      qmatch_goalsub_abbrev_tac ‘ffi_divg_stream conf nstY param chnks’ >>
+      ‘ffi_divg_stream conf nstX param chnks ⇔
+        ffi_divg_stream conf nstY param chnks’
+        suffices_by metis_tac[] >>
+      first_x_assum irule >>
+      MAP_EVERY qunabbrev_tac [‘nstX’,‘nstY’] >>
+      fs[] >> qabbrev_tac ‘XP = (XP1,XP2,XP3)’ >>
+      first_x_assum (K ALL_TAC) >>
+      rw[] >>
+      ‘XP0 = h’
+        suffices_by (rw[] >> metis_tac[strans_pres_wf,ffi_eq_pres]) >>
+      metis_tac[ffi_eq_ARecv])
+  >- (fs[pairTheory.FORALL_PROD] >>
+      qmatch_goalsub_rename_tac ‘¬strans conf _ (ARecv _ MO) _’ >>
+      first_x_assum (qspec_then ‘MO’ assume_tac) >>
+      fs[GSYM pairTheory.FORALL_PROD] >>
+      metis_tac[ffi_eq_def,BISIM_REL_def,BISIM_def])
+  >- (rename1 ‘(λ(m,ns). strans _ _ (ARecv param m) ns) XP’ >>
+      PairCases_on ‘XP’ >>
+      fs[] >> rw[]
+      >- metis_tac[ffi_eq_ARecv] >>
+      qmatch_asmsub_abbrev_tac  ‘ffi_divg_stream conf nstX param chnks’ >>
+      qmatch_goalsub_abbrev_tac ‘ffi_divg_stream conf nstY param chnks’ >>
+      ‘ffi_divg_stream conf nstX param chnks ⇔
+        ffi_divg_stream conf nstY param chnks’
+        suffices_by metis_tac[] >>
+      first_x_assum irule >>
+      MAP_EVERY qunabbrev_tac [‘nstX’,‘nstY’] >>
+      fs[] >> qabbrev_tac ‘XP = (XP1,XP2,XP3)’ >>
+      first_x_assum (K ALL_TAC) >>
+      rw[] >>
+      ‘XP0 = h’
+        suffices_by (rw[] >> metis_tac[strans_pres_wf,ffi_eq_pres,ffi_eq_equivRel,
+                                       equivalence_def,symmetric_def]) >>
+      metis_tac[ffi_eq_ARecv])
+  >- (fs[pairTheory.FORALL_PROD] >>
+      qmatch_goalsub_rename_tac ‘¬strans conf _ (ARecv _ MO) _’ >>
+      first_x_assum (qspec_then ‘MO’ assume_tac) >>
+      fs[GSYM pairTheory.FORALL_PROD] >>
+      metis_tac[ffi_eq_def,BISIM_REL_def,BISIM_def])
+QED 
+
+Definition ffi_fail_stream_def:
+  (ffi_fail_stream conf st src (c1::cs) =
+    (¬final c1 ∧
+    ∀s param bytes.
+      valid_receive_call_format conf src s param bytes ⇒
+      ∃nst.
+        call_FFI st s param bytes = FFI_return nst c1 ∧
+        ffi_fail_stream conf nst src cs)) ∧
+  (ffi_fail_stream conf st src [] =
+    ∀s param bytes.
+      valid_receive_call_format conf src s param bytes ⇒
+        call_FFI st s param bytes = FFI_final(Final_event s param bytes FFI_failed))
+End
+
+Theorem ffi_eq_fail_stream:
+  ∀conf x y.
+    ffi_wf x.ffi_state ∧
+    ffi_wf y.ffi_state ∧
+    x.oracle = comms_ffi_oracle conf ∧
+    y.oracle = comms_ffi_oracle conf ∧
+    ffi_eq conf x.ffi_state y.ffi_state ⇒
+    ffi_fail_stream conf x = ffi_fail_stream conf y
+Proof
+  simp[FUN_EQ_THM,PULL_FORALL] >>
+  rpt gen_tac >>
+  rename1 ‘ffi_fail_stream conf x src chnks = ffi_fail_stream conf y src chnks’ >>
+  MAP_EVERY qid_spec_tac [‘y’,‘x’] >>
+  Induct_on ‘chnks’
+  >- (rw[ffi_fail_stream_def,EQ_IMP_THM] >>
+      first_x_assum (drule_all_then strip_assume_tac) >>
+      rfs[call_FFI_def,ffi_receive_def,valid_receive_call_format_def,
+         comms_ffi_oracle_def,AllCaseEqs()] >>
+      first_x_assum mp_tac >>
+      ntac 2 (DEEP_INTRO_TAC some_intro) >>
+      rw[pairTheory.EXISTS_PROD]
+      >- (rename1 ‘(λ(m,ns). strans _ _ (ARecv param m) ns) XP’ >>
+          PairCases_on ‘XP’ >>
+          fs[] >> qmatch_asmsub_rename_tac ‘LENGTH BM ≠ SUC conf.payload_size’ >>
+          ‘XP0 = BM’
+            suffices_by rw[] >>
+          qmatch_asmsub_abbrev_tac ‘strans conf y.ffi_state _ TI’ >>
+          metis_tac[ffi_eq_ARecv])
+      >- (fs[pairTheory.FORALL_PROD] >>
+          qmatch_goalsub_rename_tac ‘¬strans conf _ (ARecv _ MO) _’ >>
+          first_x_assum (qspec_then ‘MO’ assume_tac) >>
+          fs[GSYM pairTheory.FORALL_PROD] >>
+          metis_tac[ffi_eq_def,BISIM_REL_def,BISIM_def])
+      >- (rename1 ‘(λ(m,ns). strans _ _ (ARecv param m) ns) XP’ >>
+          PairCases_on ‘XP’ >>
+          fs[] >> qmatch_asmsub_rename_tac ‘LENGTH BM ≠ SUC conf.payload_size’ >>
+          ‘XP0 = BM’
+            suffices_by rw[] >>
+          qmatch_asmsub_abbrev_tac ‘strans conf x.ffi_state _ TI’ >>
+          metis_tac[ffi_eq_ARecv])
+      >- (fs[pairTheory.FORALL_PROD] >>
+          qmatch_goalsub_rename_tac ‘¬strans conf _ (ARecv _ MO) _’ >>
+          first_x_assum (qspec_then ‘MO’ assume_tac) >>
+          fs[GSYM pairTheory.FORALL_PROD] >>
+          metis_tac[ffi_eq_def,BISIM_REL_def,BISIM_def])) >>
+  rw[ffi_fail_stream_def, EQ_IMP_THM] >>
+  first_x_assum (drule_all_then strip_assume_tac) >>
+  rfs[call_FFI_def,ffi_receive_def,valid_receive_call_format_def,
+         comms_ffi_oracle_def,AllCaseEqs()] >>
+  qpat_x_assum ‘(some (m,ns). strans conf _ (ARecv _ m) ns) = _’ mp_tac >>
+  ntac 2 (DEEP_INTRO_TAC some_intro) >>
+  rw[pairTheory.EXISTS_PROD]
+  >- (rename1 ‘(λ(m,ns). strans _ _ (ARecv param m) ns) XP’ >>
+      PairCases_on ‘XP’ >>
+      fs[] >> rw[]
+      >- metis_tac[ffi_eq_ARecv] >>
+      qmatch_asmsub_abbrev_tac  ‘ffi_fail_stream conf nstX param chnks’ >>
+      qmatch_goalsub_abbrev_tac ‘ffi_fail_stream conf nstY param chnks’ >>
+      ‘ffi_fail_stream conf nstX param chnks ⇔
+        ffi_fail_stream conf nstY param chnks’
+        suffices_by metis_tac[] >>
+      first_x_assum irule >>
+      MAP_EVERY qunabbrev_tac [‘nstX’,‘nstY’] >>
+      fs[] >> qabbrev_tac ‘XP = (XP1,XP2,XP3)’ >>
+      first_x_assum (K ALL_TAC) >>
+      rw[] >>
+      ‘XP0 = h’
+        suffices_by (rw[] >> metis_tac[strans_pres_wf,ffi_eq_pres]) >>
+      metis_tac[ffi_eq_ARecv])
+  >- (fs[pairTheory.FORALL_PROD] >>
+      qmatch_goalsub_rename_tac ‘¬strans conf _ (ARecv _ MO) _’ >>
+      first_x_assum (qspec_then ‘MO’ assume_tac) >>
+      fs[GSYM pairTheory.FORALL_PROD] >>
+      metis_tac[ffi_eq_def,BISIM_REL_def,BISIM_def])
+  >- (rename1 ‘(λ(m,ns). strans _ _ (ARecv param m) ns) XP’ >>
+      PairCases_on ‘XP’ >>
+      fs[] >> rw[]
+      >- metis_tac[ffi_eq_ARecv] >>
+      qmatch_asmsub_abbrev_tac  ‘ffi_fail_stream conf nstX param chnks’ >>
+      qmatch_goalsub_abbrev_tac ‘ffi_fail_stream conf nstY param chnks’ >>
+      ‘ffi_fail_stream conf nstX param chnks ⇔
+        ffi_fail_stream conf nstY param chnks’
+        suffices_by metis_tac[] >>
+      first_x_assum irule >>
+      MAP_EVERY qunabbrev_tac [‘nstX’,‘nstY’] >>
+      fs[] >> qabbrev_tac ‘XP = (XP1,XP2,XP3)’ >>
+      first_x_assum (K ALL_TAC) >>
+      rw[] >>
+      ‘XP0 = h’
+        suffices_by (rw[] >> metis_tac[strans_pres_wf,ffi_eq_pres,ffi_eq_equivRel,
+                                       equivalence_def,symmetric_def]) >>
+      metis_tac[ffi_eq_ARecv])
+  >- (fs[pairTheory.FORALL_PROD] >>
+      qmatch_goalsub_rename_tac ‘¬strans conf _ (ARecv _ MO) _’ >>
+      first_x_assum (qspec_then ‘MO’ assume_tac) >>
+      fs[GSYM pairTheory.FORALL_PROD] >>
+      metis_tac[ffi_eq_def,BISIM_REL_def,BISIM_def])
+QED 
+
+
+Theorem ffi_gets_stream:
+  ∀conf src (st : total_state ffi_state).
+    ffi_wf st.ffi_state ∧
+    st.oracle = comms_ffi_oracle conf ⇒
+    ((∃cs. ffi_term_stream conf st src cs) ∨
+     (∃cs. ffi_divg_stream conf st src cs) ∨
+     (∃cs. ffi_fail_stream conf st src cs))
+Proof
+  cheat
+(*
+  rw[] >>
+  reverse (Induct_on ‘qlk ((λ(_,q,_).q) st.ffi_state) src’)
+  >- (rw[] >> qabbrev_tac ‘fs = st.ffi_state’ >>
+      PairCases_on ‘fs’ >> rename1 ‘(c,q,N)’ >> rename1 ‘h::tl’ >>
+      first_x_assum (qspecl_then [‘st with ffi_state := (c,q |+ (src,tl),N)’,‘src’] assume_tac) >>
+      Cases_on ‘LENGTH h ≠ SUC conf.payload_size’
+      >- (ntac 2 DISJ2_TAC >> qexists_tac ‘[]’ >>
+          rw[ffi_fail_stream_def,call_FFI_def,
+              valid_receive_call_format_def,comms_ffi_oracle_def,
+              ffi_receive_def] >>
+          DEEP_INTRO_TAC some_intro >>
+          rw[]
+          >- (rename1 ‘case x of (m,ns) => _’ >>
+              PairCases_on ‘x’ >> fs[strans_rules] >>
+              ‘∃s2. strans conf (c,q,N) (ARecv src h) s2’
+                suffices_by metis_tac[functional_ARecv] >>
+              metis_tac[strans_rules])
+          >- (fs[strans_rules] >>
+              ‘∃s2. strans conf (c,q,N) (ARecv src h) s2’
+                by metis_tac[strans_rules] >>
+              qexists_tac ‘(h,s2)’ >> rw[])) >>
+      Cases_on ‘final h’ >>
+      >- (DISJ1_TAC >> qexists_tac ‘[h]’ >>
+          rw[ffi_term_stream_def,call_FFI_def,valid_receive_call_format_def,
+             comms_ffi_oracle_def, ffi_receive_def] >>
+          DEEP_INTRO_TAC some_intro >>
+          rw[]
+          >- (rename1 ‘case x of (m,ns) => _’ >>
+              PairCases_on ‘x’ >> fs[strans_rules] >>
+              ‘∃s2. strans conf (c,q,N) (ARecv src h) s2’
+                suffices_by metis_tac[functional_ARecv] >>
+              metis_tac[strans_rules])
+          >- (fs[strans_rules] >>
+              ‘∃s2. strans conf (c,q,N) (ARecv src h) s2’
+                by metis_tac[strans_rules] >>
+              qexists_tac ‘(h,s2)’ >> rw[])) >>
+      rfs[ffi_wf_def]
+      >- (DISJ1_TAC >> qexists_tac ‘h::cs’ >>
+          Cases_on ‘cs’ >>
+          rw[ffi_term_stream_def,call_FFI_def,valid_receive_call_format_def,
+             comms_ffi_oracle_def, ffi_receive_def] >>
+          fs[ffi_term_stream_def] >>
+          DEEP_INTRO_TAC some_intro >>
+          rw[]
+          >- (rename1 ‘case x of (m,ns) => _’ >>
+              PairCases_on ‘x’ >> fs[strans_rules] >>
+              ‘x0 = h’
+                suffices_by rw[]
+              ‘strans conf (c,q,N) (ARecv src h) (c,q |+ (src,tl),N)’
+                suffices_by metis_tac[functional_ARecv] >>
+              metis_tac[strans_rules])
+
+
+          rw[Once ffi_term_stream_def] >>
+          )
+
+          fs[Once strans_cases]
+          >- (first_x_assum (assume_tac o GSYM) >>
+              last_x_assum (assume_tac o GSYM) >>
+              fs[])
+          strans_ind
+      rfs[ffi_wf_def]
+      >- (DISJ1_TAC >> Cases_on ‘final h’
+          >- (qexists_tac ‘[h]’ >>
+              rw[ffi_term_stream_def,call_FFI_def,valid_receive_call_format_def,
+                 comms_ffi_oracle_def,ffi_receive_def] >>
+              DEEP_INTRO_TAC some_intro >>
+              rw[]
+              >- (rename1 ‘case x of (m,ns) => _’ >>
+                  PairCases_on ‘x’ >> fs[strans_rules] >>
+                  ‘LENGTH x0 = SUC conf.payload_size’
+                    suffices_by (rw[])
+              >- (‘(λ(m,ns). strans conf (c,q,N) (ARecv src m) ns) (h,(c,q |+ (src,tl),N))’
+                    suffices_by metis_tac[] >>
+                  rw[strans_rules]) >>
+              SELECT_ELIM_TAC)
+      Induct_on ‘qlk q src’ >> rw[]
+      >- (cheat) >>
+      rename1 ‘h::tl’ >>
+      first_x_assum (qspecl_then [‘q |+ (src,tl)’,‘src’] assume_tac) >>
+
+      Cases_on ‘st.ffi_state’ >> rename1 ‘(q,r)’ >>
+      Cases_on ‘qlk q src’
+      rw[] >>
+      Cases_on ‘∃cs. ffi_divg_stream conf st src cs’ >> 
+      rw[] >>
+      fs[ffi_term_stream_def,ffi_divg_stream_def] >>
+      CCONTR_TAC >> rw[] >> fs[] >> 
+*)
+QED
+
+val _ = export_theory ();
