projection/proofs/to_cake/payload_to_cakemlProofScript.sml
@@ -5,7 +5,8 @@ open endpoint_to_payloadTheory;
 open payloadLangTheory payloadSemTheory payload_to_cakemlTheory;
 open comms_ffi_modelTheory
      comms_ffi_propsTheory
-     comms_ffi_eqTheory;
+     comms_ffi_eqTheory
+     comms_ffi_rec_characTheory;
 open evaluate_toolsTheory
      ckExp_EquivTheory;
 open evaluate_rwLib
@@ -1222,6 +1223,7 @@ Proof
 QED
 
 (* Main receiveloop characterisation *)
+
 Theorem receiveloop_correct:
   ∀conf l env env' s src bufLoc bufInit.
     (* We have a sensible environment for execution at all *)
@@ -1464,6 +1466,33 @@ Proof
           rw[] >> SELECT_ELIM_TAC >> rw[])
       >- rw[LIST_TYPE_def,list_type_num_def])
 QED
+
+Theorem receiveloop_pres_ffi_eq:
+  ∀conf env env' s1 s2 src bufLoc bufInit.
+    (* We have a sensible environment for execution at all *)
+    env_asm env' conf ∧
+    conf.payload_size ≠ 0 ∧
+    (* Receive loop function and storage buffer properly initialised *)
+    nsLookup env.v (Short "receiveloop") = SOME(Recclosure env' (receiveloop conf (MAP (CHR o w2n) src)) "receiveloop") ∧
+    nsLookup env'.v (Short "buff") = SOME(Loc bufLoc) ∧
+    store_lookup bufLoc s1.refs = SOME(W8array bufInit) ∧
+    store_lookup bufLoc s2.refs = SOME(W8array bufInit) ∧
+    LENGTH bufInit = SUC conf.payload_size ∧
+    (* Our ffi is in the right state to receive the same message *)
+    ffi_eq conf s1.ffi.ffi_state s2.ffi.ffi_state
+    ⇒
+    ∃ckA1 ckB1 ckA2 ckB2 refsB1 refsB2 ffiB1 ffiB2 r1 r2.
+    evaluate$evaluate (s1 with clock:= ckA1) env [App Opapp [Var (Short "receiveloop"); Con NONE []]] =
+                      (s1 with <|clock := ckB1; refs := refsB1; ffi:= ffiB1|>,
+                      r1) ∧
+    evaluate$evaluate (s2 with clock:= ckA2) env [App Opapp [Var (Short "receiveloop"); Con NONE []]] =
+                      (s2 with <|clock := ckB2; refs := refsB2; ffi:= ffiB2|>,
+                      r2) ∧
+    ffi_eq conf ffiB1.ffi_state ffiB2.ffi_state ∧
+    (r1 = r2)
+Proof
+  cheat
+QED        
 
 (* HOL HELPERS CORRECT *)
 Theorem w1ckV_is_1w:
@@ -2303,7 +2332,22 @@ Proof
       simp[] >> first_x_assum (K ALL_TAC) >>
       rw[cEval_equiv_def])
   >- ((* Receive Case *)
-      cheat)
+      qabbrev_tac ‘rec = App Opapp [Var (Short "receiveloop"); Con NONE []]’ >>
+      qabbrev_tac ‘lsa = App Opapp [App Opapp [Var conf.append; rec]; convDatumList conf l]’ >>
+      qabbrev_tac ‘lsc = App Opapp [Var conf.concat; lsa]’ >>
+      rw (buffer_size_def::eval_sl) >>
+      rename1 ‘ALL_DISTINCT
+                   (MAP (λ(x,y,z). x) (receiveloop conf (MAP (CHR ∘ w2n) l0)))’ >>
+      ‘ALL_DISTINCT
+                   (MAP (λ(x,y,z). x) (receiveloop conf (MAP (CHR ∘ w2n) l0)))’
+        by rw[receiveloop_def,ALL_DISTINCT] >>
+      rw[] >> pop_assum (K ALL_TAC) >>
+      MAP_EVERY qunabbrev_tac [‘lsa’,‘lsc’] >>
+      (* Evaluate Left Hand Side *)
+      ntac 4 (rw[Once evaluate_def]) >>
+      qmatch_goalsub_abbrev_tac ‘evaluate (cSt1M with clock := _) cEnvM’ >>
+      cheat
+      )
   >- ((* IfThen case *)
       ‘∃ha_s. FLOOKUP pSt.bindings s = SOME ha_s’
         by fs[cpEval_valid_def,pSt_pCd_corr_def] >>
